\documentclass[11pt]{article}
\usepackage{amsthm}
\usepackage{amssymb}
\usepackage{amsmath}

\newtheorem{prf}{}

\title{Proof of a limit}
\author{José Ramírez}
\begin{document}
\maketitle

\begin{prf}
Suppose we have a sequence $a_n$ with a parmeter $k \ge 1$ with the following recurrence:
$$
	a_n = \frac{a_{n - 1} + \dots + a_{n - k}}{k}
$$
for all $n \ge k$. Then, we have:
$$
	\lim_{n \to \infty} a_n = \frac{2a_1}{k(k + 1)} + \frac{4a_2}{k(k + 1)} + \cdots + \frac{2ka_k}{k(k + 1)}.
$$
\end{prf}

\noindent {\bf Proof:}

From the recurrence formula, we see that the following equations hold $\forall m \in [k + 1, n]$:
$$
	ka_m = a_{m - k} + \cdots + a_{m - 1}.
$$


Here we have $n - k$ equations total; summing them all up, we arrive at an equation like this one:
$$
	r_{k + 1}a_{k + 1} + \cdots + r_na_n = r_1a_1 + \cdots + r_ka_k.
$$

Now, what are the $r_i$?

We see that, for $j \ge k + 1$, $a_j$ appears $((n - k) - (j - k + 1) + 1) = n - j$ times on the RHS through all the sums, and so it's RHS coefficient is $n - j$.
On the other hand, it's LHS coefficient is just $k$. So, after simplifying the equation, $r_j = k + j - n$ for $j \ge k + 1$.

Analogously, for $j \le k$, we see that $r_j = j$. Which leads us to the following:
$$
	a_{k + 1} + 2a_{k + 2} + \cdots + ka_n = a_1 + \cdots + ka_k.
$$

Now, if we let $\lim_{n \to \infty}a_n = L$, we can take the limit as $n \to \infty$, and get the following:

\begin{eqnarray*}
	L + 2L + \cdots + kL = a_1 + \cdots + ka_k\\
	\frac{k(k + 1)}{2}L = a_1 + \cdots + ka_k\\
	L = \frac{2}{k(k + 1)}(a_1 + \cdots + ka_k)\\
	L = \frac{2a_1}{k(k + 1)} + \frac{4a_2}{k(k + 1)} + \cdots + \frac{2ka_k}{k(k + 1)}
\end{eqnarray*}

\end{document}