\documentclass{book}
\usepackage{amsmath,amssymb,latexsym}
\begin{document}
	Using Stewart's theorem, we get the following:
	$$
		BD+4CD=3CD((2AD)^2+BD \times CD)
	$$
	so, using that $2=\frac{AB}{AC}=\frac{BD}{CD}\,$we get
	the first equation becomes
	$$
		6CD=3CD(6CD^2),
	$$
	or equivalently: $CD=\frac{1}{\sqrt{3}};\;\;$hence $BC=3CD=\sqrt{3}.$
	So, by Hero's formula, we get the area of ABC as follows:
	$$
		 p=\frac{2+1+\sqrt{3}}{2}=\frac{3+\sqrt{3}}{2};
	$$
	$$
		 a=BC=\sqrt{3}; b=AC=1; c=AB=2;
	$$
	and so:
	$$
		(ABC)=\sqrt{p(p-a)(p-b)(p-c)}=
	$$
	$$
		\sqrt{\left(\frac{3+\sqrt{3}}{2}\right)\left(\frac{3-\sqrt{3}}{2}\right)\left(\frac{1+\sqrt{3}}{2}\right)\left(\frac{\sqrt{3}-1}{2}\right)}=								\sqrt{\left(\frac{6}{4}\right)\left(\frac{2}{4}\right)}=\frac{\sqrt{3}}{2}
	$$
\end{document}